Cleanup after changing representation of interpretation of context

prelude/base.v
@@ -7,8 +7,31 @@ From iris.prelude Require Export prelude.
 Global Set Bullet Behavior "Strict Subproofs".
 Global Open Scope general_if_scope.
 Ltac done := prelude.tactics.done.
+Require Export Autosubst.Autosubst.
 
+Fixpoint iter (n : nat) `(f : A → A) :=
+  match n with
+  | O => λ x, x
+  | S n' => λ x, f (iter n' f x)
+  end.
 
+Section Autosubst_Lemmas.
+  Context {term : Type} {Ids_term : Ids term}
+          {Rename_term : Rename term} {Subst_term : Subst term}
+          {SubstLemmas_term : SubstLemmas term}.
+  
+  Lemma iter_up (m x : nat) (f : var → term) :
+    iter m up f x = if lt_dec x m then ids x else rename (+m) (f (x - m)).
+  Proof.
+    revert x; induction m; cbn; auto with omega.
+    intros x; destruct x; cbn; asimpl; trivial.
+    intros x; destruct x; cbn; asimpl; trivial.
+    rewrite IHm; repeat destruct lt_dec;
+      asimpl; auto with omega.
+  Qed.
+
+End Autosubst_Lemmas.
+  
 Section uPred_Lemmas.
   Import uPred.
   Context {Λ : language} {Σ : iFunctor}.
